src/Ex/MsiSvTwo.v
@@ -64,7 +64,7 @@ Section System.
              MsgsFrom [ec coidx]
              /\oprec MsgIdsFrom [getRq]
              /\oprec RqAccepting
-             /\oprec LockFree0
+             /\oprec UpLockFree0
              /\oprec
                  fun (ost: OState ImplOStateIfc) orq mins =>
                    ost#[implStatusIdx] >= msiS;
@@ -83,7 +83,7 @@ Section System.
              MsgsFrom [ec coidx]
              /\oprec MsgIdsFrom [getRq]
              /\oprec RqAccepting
-             /\oprec LockFree0
+             /\oprec UpLockFree0
              /\oprec
                  fun (ost: OState ImplOStateIfc) orq mins =>
                    ost#[implStatusIdx] = msiI;
@@ -124,8 +124,7 @@ Section System.
            rule_precond :=
              MsgsFrom [pc coidx]
              /\oprec MsgIdsFrom [msiDownRqS]
-             /\oprec RqAccepting
-             /\oprec HalfLockFree0;
+             /\oprec RqAccepting;
            rule_trs :=
              fun (ost: OState ImplOStateIfc) orq mins =>
                (ost+#[implStatusIdx <- msiS],
@@ -141,7 +140,7 @@ Section System.
              MsgsFrom [ec coidx]
              /\oprec MsgIdsFrom [setRq]
              /\oprec RqAccepting
-             /\oprec LockFree0
+             /\oprec UpLockFree0
              /\oprec
                  fun (ost: OState ImplOStateIfc) orq mins =>
                    ost#[implStatusIdx] = msiM;
@@ -166,7 +165,7 @@ Section System.
              MsgsFrom [ec coidx]
              /\oprec MsgIdsFrom [setRq]
              /\oprec RqAccepting
-             /\oprec LockFree0
+             /\oprec UpLockFree0
              /\oprec
                  fun (ost: OState ImplOStateIfc) orq mins =>
                    ost#[implStatusIdx] <> msiM;
@@ -208,8 +207,7 @@ Section System.
            rule_precond :=
              MsgsFrom [pc coidx]
              /\oprec MsgIdsFrom [msiDownRqM]
-             /\oprec RqAccepting
-             /\oprec HalfLockFree0;
+             /\oprec RqAccepting;
            rule_trs :=
              fun (ost: OState ImplOStateIfc) orq mins =>
                (ost +#[implStatusIdx <- msiI],
@@ -223,7 +221,7 @@ Section System.
         {| rule_idx := 8;
            rule_precond :=
              RqAccepting
-             /\oprec LockFree0
+             /\oprec UpLockFree0
              /\oprec
                  fun (ost: OState ImplOStateIfc) orq mins =>
                    ost#[implStatusIdx] <> msiI;
@@ -285,7 +283,7 @@ Section System.
                MsgsFrom [cpRq coidx]
                /\oprec MsgIdsFrom [msiRqS]
                /\oprec RqAccepting
-               /\oprec LockFree0
+               /\oprec DownLockFree0
                /\oprec
                    fun (ost: OState ImplOStateIfc) orq mins =>
                      ost#[implStatusIdx] <= msiS;
@@ -308,7 +306,7 @@ Section System.
                MsgsFrom [cpRq coidx]
                /\oprec MsgIdsFrom [msiRqS]
                /\oprec RqAccepting
-               /\oprec LockFree0
+               /\oprec DownLockFree0
                /\oprec
                    fun (ost: OState ImplOStateIfc) orq mins =>
                      ost#[implStatusIdx] = msiM;
@@ -357,7 +355,7 @@ Section System.
                MsgsFrom [cpRq coidx]
                /\oprec MsgIdsFrom [msiRqM]
                /\oprec RqAccepting
-               /\oprec LockFree0
+               /\oprec DownLockFree0
                /\oprec
                    fun (ost: OState ImplOStateIfc) orq mins =>
                      ost#[implStatusIdx] = msiI;
@@ -376,7 +374,7 @@ Section System.
                MsgsFrom [cpRq coidx]
                /\oprec MsgIdsFrom [msiRqM]
                /\oprec RqAccepting
-               /\oprec LockFree0
+               /\oprec DownLockFree0
                /\oprec
                    fun (ost: OState ImplOStateIfc) orq mins =>
                      ost#[implStatusIdx] <> msiI;
@@ -421,7 +419,7 @@ Section System.
                MsgsFrom [cpRq coidx]
                /\oprec MsgIdsFrom [msiRqI]
                /\oprec RqAccepting
-               /\oprec LockFree0
+               /\oprec DownLockFree0
                /\oprec
                    fun (ost: OState ImplOStateIfc) orq mins =>
                      ost#[implStatusIdx] = msiS;
@@ -444,7 +442,7 @@ Section System.
                MsgsFrom [cpRq coidx]
                /\oprec MsgIdsFrom [msiRqI]
                /\oprec RqAccepting
-               /\oprec LockFree0
+               /\oprec DownLockFree0
                /\oprec
                    fun (ost: OState ImplOStateIfc) orq mins =>
                      ost#[implStatusIdx] = msiM;
